Semantic/Stlc/Denotation.lean
@@ -10,6 +10,7 @@ def Ty.val_denot : Ty -> Exp 0 -> Prop
 | .nat => fun e  =>
   e.IsNumVal
 | .arrow T U => fun e =>
+  e.IsVal ∧
   ∀ arg_v,
     Ty.val_denot T arg_v ->
     Ty.exp_denot U (.app e arg_v)
@@ -22,9 +23,33 @@ def Ty.exp_denot : Ty -> Exp 0 -> Prop
 
 end
 
--- def SemanticTyping (Γ : Ctx n) (e : Exp n) (T : Ty) : Prop :=
---   ∀ s,
---     TypedStore s Γ ->
---     Ty.exp_denot T ⟨s, e⟩
+inductive Store : Nat -> Type where
+| nil : Store 0
+| cons : (e : Exp 0) -> (hv : e.IsVal) -> Store n -> Store (n + 1)
 
--- notation:65 Γ " ⊨ " e " : " T => SemanticTyping Γ e T
+def Store.lookup : Store n -> Var n -> Exp 0
+| .cons v _ s, .here => v
+| .cons _ _ s, .there i => s.lookup i
+
+def TypedStore : Store n -> Ctx n -> Prop
+| .nil, .empty => True
+| .cons v _ s, .var Γ T =>
+  Ty.val_denot T v ∧ TypedStore s Γ
+
+def Subst.fromStore (s : Store n) : Subst n 0 where
+  exp := fun x => s.lookup x
+
+def SemanticTyping (Γ : Ctx n) (e : Exp n) (T : Ty) : Prop :=
+  ∀ s,
+    TypedStore s Γ ->
+    Ty.exp_denot T (e.subst (Subst.fromStore s))
+
+notation:65 Γ " ⊨ " e " : " T => SemanticTyping Γ e T
+
+theorem Store.lookup_is_val {s : Store n} :
+  (s.lookup x).IsVal := by
+  induction x
+  case here => cases s; aesop
+  case there ih =>
+    cases s; simp [Store.lookup]
+    exact ih
