Semantic/Stlc/Soundness.lean
@@ -1,19 +1,33 @@
 import Semantic.Stlc.TypeSystem
-import Semantic.Stlc.Interpreter
 import Semantic.Stlc.Denotation
 import Mathlib.Tactic
+
+theorem eval_num_val {v : Exp 0}
+  (hv : v.IsNumVal) :
+  Eval v v := by
+  induction hv <;> grind [Eval]
+
+theorem eval_val {v : Exp 0}
+  (hv : v.IsVal) :
+  Eval v v := by
+  cases hv <;> try grind [Eval]
+  case bool hv => cases hv <;> grind [Eval]
+  case num hv => apply eval_num_val hv
 
 theorem typed_store_lookup
   (hts : TypedStore s Γ)
   (hb : Ctx.Lookup Γ x T) :
-  Ty.val_denot T ⟨s, s.lookup x⟩ := by
+  Ty.val_denot T (s.lookup x) := by
   induction hb
   case here =>
     cases s; rename_i s0 v0
     simp [TypedStore] at hts
     simp [Store.lookup]
-    sorry
-  case there ih => sorry
+    aesop
+  case there ih =>
+    cases s; simp only [Store.lookup]
+    cases hts
+    grind
 
 theorem sem_typ_var
   (hb : Ctx.Lookup Γ x T) :
@@ -22,8 +36,9 @@ theorem sem_typ_var
   simp [Ty.exp_denot]
   use s.lookup x
   split_ands
-  { grind [Eval] }
-  { sorry }
+  { apply eval_val
+    apply Store.lookup_is_val }
+  { apply typed_store_lookup hts hb }
 
 theorem sem_typ_nsucc
   (ht : Γ ⊨ e : Ty.nat) :
@@ -35,15 +50,44 @@ theorem sem_typ_nsucc
   simp [Ty.val_denot] at hv0
   use .nsucc v0
   split_ands
-  { grind [Eval] }
+  { grind [Exp.subst, Eval] }
   { simp [Ty.val_denot]
-    grind [Exp.is_num_val] }
+    grind [Exp.IsNumVal] }
+
+theorem val_denot_is_val
+  (hv : Ty.val_denot T v) :
+  v.IsVal := by
+  cases T
+  case bool => simp [Ty.val_denot] at hv; grind [Exp.IsVal]
+  case nat => simp [Ty.val_denot] at hv; grind [Exp.IsVal]
+  case arrow => simp [Ty.val_denot] at hv; exact hv.left
+
+theorem sem_typ_abs
+  (ht : (Γ,x:T) ⊨ e : U) :
+  (Γ ⊨ .abs T e : Ty.arrow T U) := by
+  intro s hts
+  simp [Ty.exp_denot]
+  simp [Exp.subst]
+  constructor; constructor
+  { apply eval_val; grind [Exp.IsVal] }
+  { simp [Ty.val_denot]
+    constructor; try grind [Exp.IsVal]
+    intro arg harg
+    unfold SemanticTyping at ht
+    have hvarg := val_denot_is_val harg
+    let s' := Store.cons arg hvarg s
+    have hts' : TypedStore s' (Γ,x:T) := by
+      unfold s'
+      simp [TypedStore]
+      aesop
+    specialize ht s' hts'
+    sorry }
 
 theorem soundness
   (ht : Γ ⊢ e : T) :
   (Γ ⊨ e : T) := by
   induction ht
-  case var => sorry
+  case var hb => apply sem_typ_var hb
   case abs => sorry
   case app => sorry
   case btrue =>
@@ -51,22 +95,22 @@ theorem soundness
     simp [Ty.exp_denot]
     use .btrue
     split_ands
-    { grind [Eval] }
-    { simp [Ty.val_denot]; rfl }
+    { grind [Exp.subst, Eval] }
+    { simp [Ty.val_denot]; grind [Exp.IsBoolVal] }
   case bfalse =>
     intro s hts
     simp [Ty.exp_denot]
     use .bfalse
     split_ands
-    { grind [Eval] }
-    { simp [Ty.val_denot]; rfl }
+    { grind [Exp.subst, Eval] }
+    { simp [Ty.val_denot]; grind [Exp.IsBoolVal] }
   case nzero =>
     intro s hts
     simp [Ty.exp_denot]
     use .nzero
     split_ands
-    { grind [Eval] }
-    { simp [Ty.val_denot]; rfl }
+    { grind [Exp.subst, Eval] }
+    { simp [Ty.val_denot]; grind [Exp.IsNumVal] }
   case nsucc ih => apply sem_typ_nsucc ih
   case pred => sorry
   case iszero => sorry
